src/Init/Data/Array/Lemmas.lean
@@ -3185,6 +3185,19 @@ theorem foldr_rel {xs : Array α} {f g : α → β → β} {a b : β} (r : β �
   rcases xs with ⟨xs⟩
   simp
 
+/-! ## Additional operations -/
+
+/-! ### leftpad -/
+
+-- We unfold `leftpad` and `rightpad` for verification purposes.
+attribute [simp] leftpad rightpad
+
+theorem size_leftpad (n : Nat) (a : α) (xs : Array α) :
+    (leftpad n a xs).size = max n xs.size := by simp; omega
+
+theorem size_rightpad (n : Nat) (a : α) (xs : Array α) :
+    (rightpad n a xs).size = max n xs.size := by simp; omega
+
 /-! Content below this point has not yet been aligned with `List`. -/
 
 /-! ### sum -/
